Made a new version of Sortable that doesn't use laziness.

ADT/Sortable.v
@@ -170,3 +170,133 @@ Proof.
 Qed.
 
 End Sortable_BottomUpMergesortWithSharing.
+
+Module Sortable_BottomUpMergesortWithSharing'.
+
+Definition Sortable (A : LinDec) : Type :=
+  nat * list (list A).
+
+Definition isValid {A : LinDec} (s : Sortable A) : Prop :=
+  Forall (sorted A) (snd s).
+
+Definition empty {A : LinDec} : Sortable A := (0, []).
+
+Require Import Div2.
+
+Function isEven (n : nat) : bool :=
+match n with
+    | 0 => true
+    | 1 => false
+    | S (S n') => isEven n'
+end.
+
+Require Import Sorting.MergeSort.
+
+Definition merge {A : LinDec} (l1 l2 : list A) : list A :=
+  Sorting.MergeSort.merge A (l1, l2).
+
+Function addSeg
+  {A : LinDec} (seg : list A) (s : Sortable A)
+  {measure fst s} : Sortable A :=
+match s with
+    | (_, []) => (1, [seg])
+    | (size, seg' :: segs') =>
+        if isEven size
+        then (length seg + size, seg :: seg' :: segs')
+        else addSeg (merge seg seg') (div2 size, segs')
+end.
+Proof.
+  destruct s; cbn; intros. inv teq. apply lt_div2.
+  destruct size; cbn in *.
+    congruence.
+    omega.
+Defined.
+
+Arguments addSeg {x} _ _.
+
+Definition add
+  {A : LinDec} (x : A) (s : Sortable A) : Sortable A :=
+    addSeg [x] s.
+
+Fixpoint sort_aux
+  {A : LinDec} (seg : list A) (segs : list (list A)) : list A :=
+match segs with
+    | [] => seg
+    | seg' :: segs' => sort_aux (merge seg seg') segs'
+end.
+
+Definition sort {A : LinDec} (s : Sortable A) : list A :=
+  let '(_, segs) := s in sort_aux [] segs.
+
+Lemma length_merge' :
+  forall (A : LinDec) (p : list A * list A),
+    length (merge (fst p) (snd p)) = length (fst p) + length (snd p).
+Proof.
+  intros. unfold merge.
+  functional induction @MergeSort.merge A p; cbn; auto.
+    destruct l1; auto.
+    rewrite MergeSort.merge_equation. dec.
+    rewrite MergeSort.merge_equation. dec. cbn in *. rewrite IHl. omega.
+Qed.
+
+Lemma length_merge :
+  forall (A : LinDec) (l1 l2 : list A),
+    length (merge l1 l2) = length l1 + length l2.
+Proof.
+  intros. pose (length_merge' _ (l1, l2)). cbn in e.
+  assumption.
+Qed.
+
+(** Lemmas for [isValid]. *)
+
+Lemma empty_isValid :
+  forall A : LinDec,
+    isValid (@empty A).
+Proof.
+  intro. compute. constructor.
+Qed.
+
+Lemma addSeg_isValid :
+  forall (A : LinDec) (seg : list A) (s : Sortable A),
+    sorted A seg -> isValid s -> isValid (addSeg seg s).
+Proof.
+  intros. functional induction @addSeg A seg s.
+    compute. auto.
+    compute. inv H0.
+    apply IHs0.
+      apply merge_sorted; cbn; inv H0.
+      inv H0.
+Qed.
+
+Lemma add_isValid :
+  forall (A : LinDec) (x : A) (s : Sortable A),
+    isValid s -> isValid (add x s).
+Proof.
+  intros. destruct s. cbn.
+  apply addSeg_isValid; auto.
+Qed.
+
+Lemma sort_aux_sorted :
+  forall (A : LinDec) (seg : list A) (segs : list (list A)),
+    sorted A seg -> Forall (sorted A) segs ->
+      sorted A (sort_aux seg segs).
+Proof.
+  intros. gen seg.
+  induction segs as [| seg' segs']; cbn; intros.
+    assumption.
+    apply IHsegs'.
+      inv H0.
+      apply merge_sorted; cbn.
+        assumption.
+        inv H0.
+Qed.
+
+Theorem sort_sorted :
+  forall (A : LinDec) (s : Sortable A),
+    isValid s -> sorted A (sort s).
+Proof.
+  destruct s. cbn. apply sort_aux_sorted.
+    constructor.
+Qed.
+
+End Sortable_BottomUpMergesortWithSharing'.
